\begin{equation}
\dot{x}  =  A x  +   B u  \quad{\text{   and   } }\quad  y  =  C x  
\label{eq:code1}
\end{equation}


\begin{equation}
x[k+1]= \phi x [k]+ \Gamma_1(D_c)u[k-1]+\Gamma_0(D_c)u[k] \quad \text{ and } \quad y[k] = C x[k]
\label{eq:code2}
\end{equation}


\begin{equation}
x[k+1]= \phi z [k]+ \Gamma_{aug}u[k] \quad \text{ and } \quad y[k] + C_{aug} z[k]
\label{eq:code3}
\end{equation}


\begin{equation}
u[k] = Kz[k] + Fr \quad \text{and} \quad K = -[ \ 0 \ 0 \ \cdots \ 1 \ ] \gamma_{aug}^{-1} H(\phi_{aug}) \quad \text{and} \quad F = \dfrac{1}{C_{aug} (I-\phi_{aug}-\Gamma_{aug}K)^{-1}\Gamma_{aug}}
\label{eq:code4}
\end{equation}